ChoicePrelude/examples/StoreExamples.v
@@ -6,9 +6,14 @@
 
 From ChoicePrelude Require Import Store.
 
-Definition ex_x : atom := 1%positive.
-Definition ex_y : atom := 2%positive.
-Definition ex_z : atom := 3%positive.
+(** Concrete atoms standing for paper variables x, y, z. *)
+Definition x_atom : atom := 1%positive.
+Definition y_atom : atom := 2%positive.
+Definition z_atom : atom := 3%positive.
+
+Local Notation "'x" := x_atom.
+Local Notation "'y" := y_atom.
+Local Notation "'z" := z_atom.
 
 Local Instance nat_valuesig : ValueSig nat := {|
   valuesig_eqdec := _;
@@ -17,17 +22,17 @@ Local Instance nat_valuesig : ValueSig nat := {|
 
 Local Notation StoreN := (gmap atom nat).
 
-Definition store_x1 : StoreN := <[ex_x := 1%nat]> ∅.
-Definition store_y2 : StoreN := <[ex_y := 2%nat]> ∅.
-Definition store_x1_y2 : StoreN := <[ex_x := 1%nat]> (<[ex_y := 2%nat]> ∅).
-Definition store_x2 : StoreN := <[ex_x := 2%nat]> ∅.
+Definition store_x1 : StoreN := <['x := 1%nat]> ∅.
+Definition store_y2 : StoreN := <['y := 2%nat]> ∅.
+Definition store_x1_y2 : StoreN := <['x := 1%nat]> (<['y := 2%nat]> ∅).
+Definition store_x2 : StoreN := <['x := 2%nat]> ∅.
 
 Example restrict_xy_to_x :
-  store_restrict store_x1_y2 ({[ex_x]}) = store_x1.
+  store_restrict store_x1_y2 ({['x]}) = store_x1.
 Proof. Admitted.
 
 Example restrict_xy_to_y :
-  store_restrict store_x1_y2 ({[ex_y]}) = store_y2.
+  store_restrict store_x1_y2 ({['y]}) = store_y2.
 Proof. Admitted.
 
 Example restrict_twice_intersection (s : StoreN) (X Y : aset) :
@@ -43,18 +48,18 @@ Example incompatible_overlapping_stores :
 Proof. Admitted.
 
 Example compatible_union_restrict_x :
-  store_restrict (store_x1 ∪ store_y2) ({[ex_x]}) = store_x1.
+  store_restrict (store_x1 ∪ store_y2) ({['x]}) = store_x1.
 Proof. Admitted.
 
 Example compatible_union_restrict_y :
-  store_restrict (store_x1 ∪ store_y2) ({[ex_y]}) = store_y2.
+  store_restrict (store_x1 ∪ store_y2) ({['y]}) = store_y2.
 Proof. Admitted.
 
 Example rename_moves_binding :
-  store_rename_atom ex_x ex_z store_x1_y2 =
-  <[ex_z := 1%nat]> (<[ex_y := 2%nat]> ∅).
+  store_rename_atom 'x 'z store_x1_y2 =
+  <['z := 1%nat]> (<['y := 2%nat]> ∅).
 Proof. Admitted.
 
 Example rename_missing_deletes_target :
-  store_rename_atom ex_z ex_y store_x1_y2 = <[ex_x := 1%nat]> ∅.
+  store_rename_atom 'z 'y store_x1_y2 = <['x := 1%nat]> ∅.
 Proof. Admitted.
